ECCA/equiv_lemmas.v
@@ -2,6 +2,53 @@ Require Export equiv.
 Require Import reduction_lemmas.
 Require Import Equivalence.
 
+Lemma Equiv_weakening:
+forall (Γ: context) (e1 e2: exp),
+(Γ ⊢ e1 ≡ e2) -> 
+forall (Δ: context) (r: ren), 
+Γ =[r]=> Δ ->
+(Δ ⊢ ([r] e1) ≡ ([r] e2)).
+Proof. induction 1; cbn; auto.
++ intros. apply aE_Step with (e:=[r]e); eauto using Reduces_weakening.
++ intros.
+  names. destruct H0. eapply aE_Reflect with (x:= applyt s _ x). unfold assumes in *. destruct H.
+  - left. apply H0 in h. names in h. apply h.
+  - right. destruct e. exists ([s] x0). apply H0 in H. names in H. apply H.
++ intros; names; auto.
++ intros. apply aE_Trans with (M':=[r]M'); auto.
++ intros. apply aE_Lam with (x:= x). auto. names. apply IHEquiv2.
+  auto. apply ctx_rename. auto.
++ intros. apply aE_Eta with (x:= x) (A:=[r] A0) (F':= [r] F') (F:=[r] F) (G:= [r] G) (G':=[r] G'). eauto using IHEquiv1. 
+  eauto using IHEquiv2. specialize IHEquiv3 with (Δ:= (Δ & x ~ Assum ([r] A0))) (r:= (r,, x)%ren).
+  names in IHEquiv3. names. cut ((@open x 0 (applyv r (closev x (free x)))) = (eId (free x))). 
+  - intro. rewrite H3 in IHEquiv3. apply IHEquiv3. apply ctx_rename. auto.
+  - names. auto.
++ intros. apply aE_Pi with (x:= x). auto. names. apply IHEquiv2.
+  auto. apply ctx_rename. auto.
++ intros. apply aE_Sig with (x:= x). auto. names. apply IHEquiv2.
+  auto. apply ctx_rename. auto.
++ intros. apply aE_Let with (x:= x) (A:= [r] A0). auto. names. apply IHEquiv2.
+  auto. apply ctx_rename. auto.
++ intros. apply aE_If with (p:=p). auto.
+  - specialize IHEquiv2 with (Δ:= (Δ & p ~ Assum (eEqv ([r] V) eTru))) (r:=(r,, p)%ren). names. names in IHEquiv2. apply IHEquiv2.
+    apply ctx_rename. auto.
+  - specialize IHEquiv3 with (Δ:= (Δ & p ~ Assum (eEqv ([r] V) eFls))) (r:=(r,, p)%ren). names. names in IHEquiv3. apply IHEquiv3.
+    apply ctx_rename. auto.
++ intros. destruct H0. apply aE_If_EtaTru with (p:=applyt s total p). unfold assumes in *. destruct H.
+  - left. apply H0 in H. names in H. apply H.
+  - right. destruct H. exists ([s] x). apply H0 in H. names in H. apply H.
++ intros. destruct H0. apply aE_If_EtaFls with (p:=applyt s total p). unfold assumes in *. destruct H.
+  - left. apply H0 in H. names in H. apply H.
+  - right. destruct H. exists ([s] x). apply H0 in H. names in H. apply H.
+Qed.
+ 
+Lemma Equiv_cons_shift:
+    forall (Γ : context) (e1 e2: exp) (A: ctxmem) (x: name),
+      Equiv Γ e1 e2 -> Equiv (Γ & x ~ A) ([^x] e1) ([^x] e2).
+Proof. intros.
+apply Equiv_weakening with (Γ:= Γ). auto. apply ctx_shift. apply ctx_id.
+Qed.
+
 Lemma equiv_refl (g: env): Reflexive (Equiv g).
 Proof.
 unfold Reflexive. intros. eapply aE_Reflex. 
