ECCA/reduction_lemmas.v
@@ -1,1 +1,58 @@
 Require Export reduction.
+
+Open Scope ECCA_scope.
+
+Lemma Steps_cons_shift: 
+forall (Γ : context) (e1 e2: exp) (A: ctxmem) (x: name),
+(Γ ⊢ e1 ⊳ e2) -> ((Γ & x ~ A) ⊢ ([^x] e1) ⊳ ([^x] e2)). 
+Proof. intros. induction H; cbn; auto.
++ apply st_ID with (A:= [^x] A1). names. apply has_rest. exists (Def e' A1). names. auto.
++ names. auto.
++ names. auto.
+Qed.
+
+Lemma Steps_weakening:
+forall (Γ: context) (e1 e2: exp), 
+(Γ ⊢ e1 ⊳ e2) -> 
+forall (Δ: context) (r: ren),
+Γ =[r]=> Δ ->
+(Δ ⊢ ([r] e1) ⊳ ([r] e2)).
+Proof.
+induction 1; cbn; auto.
++ intros. destruct H0. apply H0 in H. names in H. rewrite applyt_is_applyv with (rn:=total). names. 
+  apply st_ID with (A:= [s] A0). auto.
++ intros. names. auto.
++ intros. names. auto.
+Qed.
+Hint Resolve Steps_weakening.
+
+
+Lemma Reduces_weakening:
+forall (Γ: context) (e1 e2: exp),
+(Γ ⊢ e1 ⊳* e2) -> 
+forall (Δ: context) (r: ren), 
+Γ =[r]=> Δ ->
+(Δ ⊢ ([r] e1) ⊳* ([r] e2)).
+Proof. induction 1; cbn; auto.
++ intros. apply R_RedR. apply Steps_weakening with (Γ := g). auto. auto.
++ intros. apply R_Trans with (e':= [r] e'); auto.
++ intros. apply R_CongLet with (A:= [r] A0) (x:= x). auto. names. apply IHReduces2.
+  apply ctx_rename. auto.
++ intros. apply R_CongLam1 with (A:= [r] A0) (x:= x). auto. names. apply IHReduces2.
+  apply ctx_rename. auto.
++ intros. apply R_CongPi with (A:= [r] A0) (x:= x). auto. names. apply IHReduces2.
+  apply ctx_rename. auto.
++ intros. apply R_CongSig with (A:= [r] A0) (x:= x). auto. names. apply IHReduces2.
+  apply ctx_rename. auto.
+Qed.
+Hint Resolve Reduces_weakening.
+
+(* Lemma Reduces_cons_shift:
+    forall (Γ : context) (e1 e2: exp) (x: name) (A: ctxmem),
+      (Γ ⊢ e1 ⊳* e2) -> ((Γ & x ~ A) ⊢ ([^x] e1) ⊳* ([^x] e2)).
+Proof.
+intros. apply Reduces_weakening with (Γ:= Γ).
+apply ctx_shift; apply ctx_id. auto.
+Qed. *)
+
+
